theories/ftlr/ReadSR.v
@@ -9,28 +9,30 @@ From cap_machine Require Import stdpp_extra.
 
 Section fundamental.
   Context
-    {Σ : gFunctors}
-      {ceriseg: ceriseG Σ}
-      {stsg : STSG Addr region_type Σ} {heapg : heapGS Σ}
-      {sealsg: sealStoreG Σ}
-      {nainv: logrel_na_invs Σ}
-      {MP: MachineParameters}
-  .
+    {Σ:gFunctors}
+    {ceriseg:ceriseG Σ} {sealsg: sealStoreG Σ}
+    {Cname : CmptNameG}
+    {stsg : STSG Addr region_type Σ} {heapg : heapGS Σ}
+    {nainv: logrel_na_invs Σ}
+    `{MP: MachineParameters}.
 
   Notation STS := (leibnizO (STS_states * STS_rels)).
   Notation STS_STD := (leibnizO (STS_std_states Addr region_type)).
-  Notation WORLD := (prodO STS_STD STS).
+  Notation CVIEW := (prodO STS_STD STS).
+  Notation WORLD := (gmapO CmptName CVIEW).
+  Implicit Types WC : CVIEW.
   Implicit Types W : WORLD.
+  Implicit Types C : CmptName.
 
-  Notation D := (WORLD -n> (leibnizO Word) -n> iPropO Σ).
-  Notation R := (WORLD -n> (leibnizO Reg) -n> iPropO Σ).
+  Notation D := (WORLD -n> (leibnizO CmptName) -n> (leibnizO Word) -n> iPropO Σ).
+  Notation R := (WORLD -n> (leibnizO CmptName) -n> (leibnizO Reg) -n> iPropO Σ).
   Implicit Types w : (leibnizO Word).
   Implicit Types interp : (D).
 
-  Lemma readsr_case (W : WORLD) (regs : leibnizO Reg)
+  Lemma readsr_case (W : WORLD) (C : CmptName) (regs : leibnizO Reg)
     (p p' : Perm) (g : Locality) (b e a : Addr)
     (w : Word) (ρ : region_type) (dst : RegName) (src : SRegName) (P:D) :
-    ftlr_instr W regs p p' g b e a w (ReadSR dst src) ρ P.
+    ftlr_instr W C regs p p' g b e a w (ReadSR dst src) ρ P.
   Proof.
     intros Hp Hsome HcorrectPC Hbae Hfp HO Hpers Hpwl Hregion Hnotrevoked Hnotfrozen Hi.
     iIntros "#IH #Hinv_interp #Hreg #Hinva #Hrcond #Hwcond #Hmono #HmonoV Hw Hsts Hown".
@@ -63,7 +65,7 @@ Section fundamental.
     iIntros "!>" (regs' retv). iDestruct 1 as (HSpec) "[Ha Hmap]".
     destruct HSpec; cycle 1.
     - iApply wp_pure_step_later; auto. iNext; iIntros "_".
-      iApply wp_value; auto. iIntros; discriminate.
+      iApply wp_value; auto.
     - by simplify_map_eq.
   Qed.
 
