theories/ftlr/Seal.v
@@ -8,35 +8,39 @@ From cap_machine.proofmode Require Import map_simpl register_tactics.
 
 Section fundamental.
   Context
-    {Σ : gFunctors}
-      {ceriseg: ceriseG Σ}
-      {stsg : STSG Addr region_type Σ} {heapg : heapGS Σ}
-      {sealsg: sealStoreG Σ}
-      {nainv: logrel_na_invs Σ}
-      {MP: MachineParameters}
-  .
+    {Σ:gFunctors}
+    {ceriseg:ceriseG Σ} {sealsg: sealStoreG Σ}
+    {Cname : CmptNameG}
+    {stsg : STSG Addr region_type Σ} {heapg : heapGS Σ}
+    {nainv: logrel_na_invs Σ}
+    `{MP: MachineParameters}.
 
   Notation STS := (leibnizO (STS_states * STS_rels)).
   Notation STS_STD := (leibnizO (STS_std_states Addr region_type)).
-  Notation WORLD := (prodO STS_STD STS).
+  Notation CVIEW := (prodO STS_STD STS).
+  Notation WORLD := (gmapO CmptName CVIEW).
+  Implicit Types WC : CVIEW.
   Implicit Types W : WORLD.
+  Implicit Types C : CmptName.
 
-  Notation D := (WORLD -n> (leibnizO Word) -n> iPropO Σ).
-  Notation R := (WORLD -n> (leibnizO Reg) -n> iPropO Σ).
+  Notation D := (WORLD -n> (leibnizO CmptName) -n> (leibnizO Word) -n> iPropO Σ).
+  Notation R := (WORLD -n> (leibnizO CmptName) -n> (leibnizO Reg) -n> iPropO Σ).
   Implicit Types w : (leibnizO Word).
   Implicit Types interp : (D).
 
   (* Proving the meaning of sealing in the LR sane *)
-  Lemma sealing_preserves_interp W sb p0 g0 b0 e0 a0:
+  Lemma sealing_preserves_interp W C sb p0 g0 b0 e0 a0:
         permit_seal p0 = true →
         withinBounds b0 e0 a0 = true →
-        fixpoint interp1 W (WSealable sb) -∗
-        fixpoint interp1 W (borrow (WSealable sb)) -∗
-        fixpoint interp1 W (WSealRange p0 g0 b0 e0 a0) -∗
-        fixpoint interp1 W (WSealed a0 sb).
+        interp W C (WSealable sb) -∗
+        interp W C (borrow (WSealable sb)) -∗
+        interp W C (WSealRange p0 g0 b0 e0 a0) -∗
+        interp W C (WSealed a0 sb).
   Proof.
     iIntros (Hpseal Hwb) "#HVsb #HVsb_borrowed #HVsr".
-    rewrite (fixpoint_interp1_eq W (WSealRange _ _ _ _ _)) (fixpoint_interp1_eq W (WSealed _ _)) /= Hpseal /interp_sb.
+    rewrite
+      (fixpoint_interp1_eq W C (WSealRange _ _ _ _ _))
+      (fixpoint_interp1_eq W C (WSealed _ _)) /= Hpseal /interp_sb.
     iDestruct "HVsr" as "[Hss _]".
     apply seq_between_dist_Some in Hwb.
     iDestruct (big_sepL_delete with "Hss") as "[HSa0 _]"; eauto.
@@ -47,10 +51,10 @@ Section fundamental.
     by iApply "HWcond".
   Qed.
 
-  Lemma seal_case (W : WORLD) (regs : leibnizO Reg)
+  Lemma seal_case (W : WORLD)(C : CmptName) (regs : leibnizO Reg)
     (p p' : Perm) (g : Locality) (b e a : Addr)
     (w : Word) (ρ : region_type) (dst r1 r2 : RegName) (P:D):
-    ftlr_instr W regs p p' g b e a w (Seal dst r1 r2) ρ P.
+    ftlr_instr W C regs p p' g b e a w (Seal dst r1 r2) ρ P.
   Proof.
     intros Hp Hsome HcorrectPC Hbae Hfp HO Hpers Hpwl Hregion Hnotrevoked Hnotfrozen Hi.
     iIntros "#IH #Hinv_interp #Hreg #Hinva #Hrcond #Hwcond #Hmono #HmonoV Hw Hsts Hown".
@@ -65,7 +69,7 @@ Section fundamental.
     destruct HSpec as [ * Hr1 Hr2 Hseal Hwb HincrPC | ]; cycle 1.
     {
       iApply wp_pure_step_later; auto. iNext; iIntros "_".
-      iApply wp_value; auto. iIntros; discriminate.
+      iApply wp_value; auto.
     }
 
     - apply incrementPC_Some_inv in HincrPC as (p''&g''&b''&e''&a''& ? & HPC & Z & Hregs') .
@@ -75,11 +79,11 @@ Section fundamental.
       { destruct (decide (PC = r1)); last auto. simplify_map_eq; auto. }
       rewrite lookup_insert_ne in Hr1; auto.
 
-      iAssert (interp W (WSealable sb)) as "#HVsb".
+      iAssert (interp W C (WSealable sb)) as "#HVsb".
       { destruct (decide (r2 = PC)) as [Heq|Heq]; simplify_map_eq; first done.
         unshelve iSpecialize ("Hreg" $! r2 _ _ Hr2); eauto.
       }
-      iAssert (interp W (borrow (WSealable sb))) as "#HVsb_borrowed".
+      iAssert (interp W C (borrow (WSealable sb))) as "#HVsb_borrowed".
       { by iApply interp_borrow_word. }
 
       iApply wp_pure_step_later; auto; iNext; iIntros "_".
@@ -89,7 +93,7 @@ Section fundamental.
       iDestruct (region_close with "[$Hstate $Hr $Ha $HmonoV Hw]") as "Hr"; eauto.
       { destruct ρ;auto;[|ospecialize (Hnotfrozen _)];contradiction. }
 
-      iApply ("IH" $! _ (<[dst := _]> (<[PC := _]> regs))
+      iApply ("IH" $! _ _ (<[dst := _]> (<[PC := _]> regs))
                with "[%] [] [Hmap] [$Hr] [$Hsts] [$Hown]")
       ; eauto.
       + intro; cbn. by repeat (rewrite lookup_insert_is_Some'; right).
